[tetris] adequacy

theories/ert_logic/adequacy.v
@@ -7,19 +7,26 @@ From iris.prelude Require Import options.
 From clutch.prelude Require Import stdpp_ext iris_ext.
 From clutch.prob_lang Require Import erasure notation.
 From clutch.common Require Export language.
-From clutch.ert_logic Require Import expected_time_credits ert_weakestpre primitive_laws.
+From clutch.ert_logic Require Import expected_time_credits ert_weakestpre problang_wp.
 From clutch.prob Require Import distribution.
 Import uPred.
 
-Fixpoint ERT k (eσ : lang.cfg) : distr prob_lang.val :=
+Fixpoint ERT k (eσ : lang.cfg) : R :=
   match k with
-  | O => dzero
+  | O => 0
   | S n =>
       match to_val eσ.1 with
-      | Some v => dret v
-      | None => dbind (ERT n) (prim_step eσ.1 eσ.2)
+      | Some v => nnreal_zero
+      | None => 1 + SeriesC (λ ρ, (prim_step eσ.1 eσ.2 ρ) * (ERT n ρ))
       end
   end.
+
+Lemma ERT_Sn n e σ :
+  to_val e = None ->
+  ERT (S n) (e, σ) = 1 + SeriesC (λ ρ : cfg, ((step (e, σ) ρ) * (ERT n ρ))%R).
+Proof.
+  simpl. by intros ->.
+Qed.
 
 
 Section adequacy.
@@ -43,200 +50,242 @@ Section adequacy.
     iIntros (???) "/=".
     iMod ("H" with "[//]"); auto.
   Qed.
+*)
 
-  Lemma ub_lift_dbind_adv' `{Countable A, Countable A'}
-    (f : A → distr A') (μ : distr A) (R : A → Prop) (T : A' → Prop) ε ε' n :
-    ⌜ 0 <= ε ⌝ -∗
-    ⌜ exists r, forall a, 0 <= ε' a <= r ⌝ -∗
-    ⌜ub_lift μ R ε⌝ -∗
-    (∀ a , ⌜R a⌝ ={∅}▷=∗^(S n) ⌜ub_lift (f a) T (ε' a)⌝) -∗
-    |={∅}▷=>^(S n) ⌜ub_lift (dbind f μ) T (ε + SeriesC (λ a : A, (μ a * ε' a)%R))⌝ : iProp Σ.
-  Proof.
-    iIntros (???) "H".
-    iApply (step_fupdN_mono _ _ _ (⌜(∀ a b, R a → ub_lift (f a) T (ε' a))⌝)).
-    { iIntros (?). iPureIntro. eapply ub_lift_dbind_adv; eauto. }
-    iIntros (???) "/=".
-    iMod ("H" with "[//]"); auto.
-  Qed.
 
-  Lemma exec_ub_erasure (e : expr) (σ : state) (n : nat) φ (ε : nonnegreal) :
+  (* Lemma foo (e1 : expr) (σ1 : state) (n : nat) (x2 : (language.cfg prob_lang) -> nonnegreal)
+     (r : R)
+     (Hr : ∀ ρ : language.cfg prob_lang, x2 ρ <= r)
+     (Hv : to_val e1 = None)
+     :
+     ((∀ (e2 : expr) (σ2 : state),
+          ⌜prim_step e1 σ1 (e2, σ2) > 0⌝ ={∅}=∗
+          |={∅}▷=> |={∅}▷=>^n ⌜ERT n (e2, σ2) <= x2 (e2, σ2)⌝)
+      ⊢
+        |={∅}▷=>^(S n)
+          ⌜1 + SeriesC (λ ρ : cfg, (prim_step e1 σ1 ρ * ERT n ρ)%R) <=
+             1 + SeriesC (λ ρ : cfg, (prim_step e1 σ1 ρ * x2 ρ)%R)⌝)%I. *)
+
+
+
+  (* Lemma ub_lift_dbind_adv' `{Countable A, Countable A'}
+       (f : A → distr A') (μ : distr A) (R : A → Prop) (T : A' → Prop) ε ε' n :
+       ⌜ 0 <= ε ⌝ -∗
+       ⌜ exists r, forall a, 0 <= ε' a <= r ⌝ -∗
+       ⌜ub_lift μ R ε⌝ -∗
+       (∀ a , ⌜R a⌝ ={∅}▷=∗^(S n) ⌜ub_lift (f a) T (ε' a)⌝) -∗
+       |={∅}▷=>^(S n) ⌜ub_lift (dbind f μ) T (ε + SeriesC (λ a : A, (μ a * ε' a)%R))⌝ : iProp Σ.
+     Proof.
+       iIntros (???) "H".
+       iApply (step_fupdN_mono _ _ _ (⌜(∀ a b, R a → ub_lift (f a) T (ε' a))⌝)).
+       { iIntros (?). iPureIntro. eapply ub_lift_dbind_adv; eauto. }
+       iIntros (???) "/=".
+       iMod ("H" with "[//]"); auto.
+     Qed. *)
+
+
+
+  Lemma ERM_erasure (e : expr) (σ : state) (n : nat) (* φ *) (x : nonnegreal) :
     to_val e = None →
-    exec_ub e σ ε (λ '(e2, σ2) ε',
-        |={∅}▷=>^(S n) ⌜ub_lift (exec n (e2, σ2)) φ ε'⌝)
-    ⊢ |={∅}▷=>^(S n) ⌜ub_lift (exec (S n) (e, σ)) φ ε⌝.
+    ERM e σ x
+          (λ '(e2, σ2) (x' : nonnegreal),
+             |={∅}▷=>^(S n) ⌜ERT n (e2, σ2) <= x'⌝)
+    ⊢ |={∅}▷=>^(S n) ⌜ERT (S n) (e, σ) <= x⌝.
+    (* exec_ub e σ ε (λ '(e2, σ2) ε',
+           |={∅}▷=>^(S n) ⌜ub_lift (exec n (e2, σ2)) φ ε'⌝)
+       ⊢ |={∅}▷=>^(S n) ⌜ub_lift (exec (S n) (e, σ)) φ ε⌝. *)
   Proof.
     iIntros (Hv) "Hexec".
     iAssert (⌜to_val e = None⌝)%I as "-#H"; [done|]. iRevert "Hexec H".
-    rewrite /exec_ub /exec_ub'.
-    set (Φ := (λ '((e1, σ1), ε''),
+    rewrite /ERM /ERM'.
+    set (Φ := (λ '((e1, σ1), x''),
                 (⌜to_val e1 = None⌝ ={∅}▷=∗^(S n)
-                 ⌜ub_lift (exec (S n) (e1, σ1)) φ ε''⌝)%I) :
+                 ⌜ERT (S n) (e1, σ1) <= x''⌝)%I) :
            prodO cfgO NNRO → iPropI Σ).
     assert (NonExpansive Φ).
     { intros m ((?&?)&?) ((?&?)&?) [[[=] [=]] [=]]. by simplify_eq. }
-    set (F := (exec_ub_pre (λ '(e2, σ2) ε',
-                   |={∅}▷=>^(S n) ⌜ub_lift (exec n (e2, σ2)) φ ε'⌝)%I)).
+    set (F := (ERM_pre (λ '(e2, σ2) x',
+                   |={∅}▷=>^(S n) ⌜ERT n (e2, σ2) <= x'⌝)%I)).
     iPoseProof (least_fixpoint_iter F Φ with "[]") as "H"; last first.
     { iIntros "Hfix %".
       by iMod ("H" $! ((_, _)) with "Hfix [//]").
     }
     clear.
-    iIntros "!#" ([[e1 σ1] ε'']). rewrite /Φ/F/exec_ub_pre.
-    iIntros " [ (%R & %ε1 & %ε2 & %Hred & (%r & %Hr) & % & %Hlift & H)|H] %Hv".
+    iIntros "!#" ([[e1 σ1] x'']). rewrite /Φ/F/ERM_pre.
+    (* iIntros " [ (%R & %x1 & %x2 & %Hred & (%r & %Hr) & % & %Hlift & H)|H] %Hv". *)
+    iIntros " (%x2 & %Hred & (%r & %Hr) & % & H) %Hv".
     - iApply step_fupdN_mono.
       { apply pure_mono.
-        eapply UB_mon_grading; eauto. }
-      rewrite exec_Sn_not_final; [|eauto].
-      iApply ub_lift_dbind_adv'.
-      + iPureIntro; apply cond_nonneg.
-      + iPureIntro. exists r. split; auto. apply cond_nonneg.
-      + done.
-      + iIntros ([] ?).
+        intros ψ. etrans. 2: apply H.
+        exact ψ. }
+      clear H x''.
+      rewrite ERT_Sn => //.
+      (* iApply ub_lift_dbind_adv'.
+         + iPureIntro; apply cond_nonneg.
+         + iPureIntro. exists r. split; auto. apply cond_nonneg.
+         + done.
+         + iIntros ([] ?). *)
+        simpl. fold cfg.
         iApply step_fupd_fupdN_S.
-        iMod ("H" $! e s with "[]") as "H";  [iPureIntro; eauto| iModIntro ].
-        iDestruct "H" as "[%R' [%ε1' [%ε2' (%Hsum' & %Hlift' & Hwand')]]]".
-        rewrite -(dret_id_left' (fun _ : () => (exec n (e, s))) tt).
-        iApply (step_fupdN_mono _ _ _ ⌜(ub_lift _ _ (ε1' + ε2')) ⌝).
-        { iIntros "%H'"; iPureIntro. eapply UB_mon_grading; eauto. }
-        iApply (ub_lift_dbind').
-        * iPureIntro; apply cond_nonneg.
-        * iPureIntro; apply cond_nonneg.
-        * iPureIntro.
-          apply total_ub_lift_implies_ub_lift in Hlift'.
-          eapply Hlift'.
-        * iIntros (? Hcont).
-          replace tt with a; [| by destruct a].
-          iSpecialize ("Hwand'" with "[]"); [iPureIntro; eauto|].
-          rewrite (dret_id_left').
-          iApply step_fupd_fupdN_S.
-          iFrame.
-          iModIntro.
-          eauto.
-    - rewrite exec_Sn_not_final; [|eauto].
-      iDestruct (big_orL_mono _ (λ _ _,
-                     |={∅}▷=>^(S n)
-                       ⌜ub_lift (prim_step e1 σ1 ≫= exec n) φ ε''⌝)%I
-                  with "H") as "H".
-      { iIntros (i α Hα%elem_of_list_lookup_2) "(% & %ε1 & %ε2 & %Hε'' & %Hleq & %Hlift & H)".
-        replace (prim_step e1 σ1) with (step (e1, σ1)) => //.
-        rewrite -exec_Sn_not_final; [|eauto].
-        iApply (step_fupdN_mono _ _ _
-                  (⌜∀ σ2 , R2 σ2 → ub_lift (exec (S n) (e1, σ2)) φ (ε2 (e1, σ2))⌝)%I).
-        - iIntros (?). iPureIntro.
-          rewrite /= /get_active in Hα.
-          apply elem_of_elements, elem_of_dom in Hα as [bs Hα].
-          erewrite (Rcoupl_eq_elim _ _ (prim_coupl_step_prim _ _ _ _ _ Hα)); eauto.
-          apply (UB_mon_grading _ _
-                   (ε1 + (SeriesC (λ ρ : language.state prob_lang, language.state_step σ1 α ρ * ε2 (e1, ρ))))) => //.
-          eapply ub_lift_dbind_adv; eauto; [by destruct ε1|].
-          destruct Hε'' as [r Hr]; exists r.
-          intros a.
-          split; [by destruct (ε2 _) | by apply Hr].
-        - iIntros (e s).
-          iApply step_fupd_fupdN_S.
-          iMod ("H" with "[//]") as "H"; iModIntro.
-          iDestruct "H" as "[%R' [%ε1' [%ε2' (%Hsum' & %Hlift' & Hwand')]]]".
-          rewrite -(dret_id_left' (fun _ : () => (exec (S n) _)) tt).
-          iApply (step_fupdN_mono _ _ _ ⌜(ub_lift _ _ (ε1' + ε2')) ⌝).
-          { iIntros "%H'"; iPureIntro. eapply UB_mon_grading; eauto. }
-          iApply (ub_lift_dbind').
-          * iPureIntro; apply cond_nonneg.
-          * iPureIntro; apply cond_nonneg.
-          * iPureIntro.
-            apply total_ub_lift_implies_ub_lift in Hlift'.
-            eapply Hlift'.
-          * iIntros (? Hcont).
-            replace tt with a; [| by destruct a].
-            iSpecialize ("Hwand'" with "[]"); [iPureIntro; eauto|].
-            rewrite (dret_id_left').
-            iApply step_fupd_fupdN_S.
-            iMod ("Hwand'" with "[//]"); iModIntro; iFrame.
-            iModIntro; eauto. }
-      iInduction (language.get_active σ1) as [| α] "IH"; [done|].
-      rewrite big_orL_cons.
-      iDestruct "H" as "[H | Ht]"; [done|].
-      by iApply "IH".
-  Qed.
-
-  Theorem wp_refRcoupl_step_fupdN (e : expr) (σ : state) (ε : nonnegreal) n φ  :
-    state_interp σ ∗ err_interp (ε) ∗ WP e {{ v, ⌜φ v⌝ }} ⊢
-    |={⊤,∅}=> |={∅}▷=>^n ⌜ub_lift (exec n (e, σ)) φ ε⌝.
-  Proof.
-    iInduction n as [|n] "IH" forall (e σ ε); iIntros "((Hσh & Hσt) & Hε & Hwp)".
-    - rewrite /exec /=.
-      destruct (to_val e) eqn:Heq.
-      + apply of_to_val in Heq as <-.
-        rewrite ub_wp_value_fupd.
-        iMod "Hwp" as "%".
-        iApply fupd_mask_intro; [set_solver|]; iIntros.
-        iPureIntro.
-        apply (UB_mon_grading _ _ 0); [apply cond_nonneg | ].
-        apply ub_lift_dret; auto.
-      + iApply fupd_mask_intro; [set_solver|]; iIntros "_".
-        iPureIntro.
-        apply ub_lift_dzero,
-        Rle_ge,
-        cond_nonneg.
-    - rewrite exec_Sn /step_or_final /=.
-      destruct (to_val e) eqn:Heq.
-      + apply of_to_val in Heq as <-.
-        rewrite ub_wp_value_fupd.
-        iMod "Hwp" as "%".
         iApply fupd_mask_intro; [set_solver|]; iIntros "_".
+
+       iApply (step_fupdN_mono _ _ _ (⌜(∀ e2 σ2, prim_step e1 σ1 (e2, σ2) > 0 → ERT n (e2, σ2) <= x2 (e2, σ2))⌝)).
+       2: { iIntros (???) "/=".
+            iMod ("H" with "[//]"); auto. }
+       simpl. iIntros (?). iPureIntro.
+       apply Rplus_le_compat_l.
+       apply SeriesC_le.
+       2:{ admit. }
+       intros [e2 σ2].
+       split.
+       + apply Rmult_le_pos.
+         1: auto.
+         clear. revert e2 σ2. induction n.
+         ++ done.
+         ++ simpl. intros. destruct (to_val e2). 1: lra.
+            assert (0 <= SeriesC (λ ρ : expr * state, prim_step e2 σ2 ρ * ERT n ρ)).
+            2: {
+              etrans. 1: eauto.
+              rewrite -{1}(Rplus_0_l (SeriesC (λ ρ : expr * state, prim_step e2 σ2 ρ * ERT n ρ))).
+              apply Rplus_le_compat_r. lra.
+            }
+            apply SeriesC_ge_0'.
+            intros.
+            apply Rmult_le_pos.
+            2: destruct x ; apply IHn.
+            auto.
+       + clear -H.
+         destruct (decide (0 < prim_step e1 σ1 (e2, σ2))%R) as [Hgt | Hngt].
+         * apply Rmult_le_compat_l => //.
+           apply H. done.
+         * destruct (decide (0 = prim_step e1 σ1 (e2, σ2))%R) as [Heq | Hneg].
+           1: { rewrite -Heq. lra. }
+           exfalso.
+           opose proof (pmf_pos (prim_step e1 σ1) (e2, σ2)).
+           lra.
+  Admitted.
+
+
+  (*       iApply (step_fupdN_mono _ _ _ ⌜(ERT _ _ <= (1 + r)) ⌝).
+           iApply fupd_mask_intro; [set_solver|]; iIntros.
+
+           iMod ("H" $! e s with "[]") as "H";  [iPureIntro; eauto| iModIntro ].
+           iDestruct "H" as "[%R' [%x1' [%x2' (%Hsum' & %Hlift' & Hwand')]]]".
+           rewrite -(dret_id_left' (fun _ : () => (exec n (e, s))) tt).
+           iApply (step_fupdN_mono _ _ _ ⌜(ub_lift _ _ (x1' + x2')) ⌝).
+           { iIntros "%H'"; iPureIntro. eapply UB_mon_grading; eauto. }
+           iApply (ub_lift_dbind').
+           * iPureIntro; apply cond_nonneg.
+           * iPureIntro; apply cond_nonneg.
+           * iPureIntro.
+             apply total_ub_lift_implies_ub_lift in Hlift'.
+             eapply Hlift'.
+           * iIntros (? Hcont).
+             replace tt with a; [| by destruct a].
+             iSpecialize ("Hwand'" with "[]"); [iPureIntro; eauto|].
+             rewrite (dret_id_left').
+             iApply step_fupd_fupdN_S.
+             iFrame.
+             iModIntro.
+             eauto.
+       - rewrite exec_Sn_not_final; [|eauto].
+         iDestruct (big_orL_mono _ (λ _ _,
+                        |={∅}▷=>^(S n)
+                          ⌜ub_lift (prim_step e1 σ1 ≫= exec n) φ x''⌝)%I
+                     with "H") as "H".
+         { iIntros (i α Hα%elem_of_list_lookup_2) "(% & %x1 & %x2 & %Hx'' & %Hleq & %Hlift & H)".
+           replace (prim_step e1 σ1) with (step (e1, σ1)) => //.
+           rewrite -exec_Sn_not_final; [|eauto].
+           iApply (step_fupdN_mono _ _ _
+                     (⌜∀ σ2 , R2 σ2 → ub_lift (exec (S n) (e1, σ2)) φ (x2 (e1, σ2))⌝)%I).
+           - iIntros (?). iPureIntro.
+             rewrite /= /get_active in Hα.
+             apply elem_of_elements, elem_of_dom in Hα as [bs Hα].
+             erewrite (Rcoupl_eq_elim _ _ (prim_coupl_step_prim _ _ _ _ _ Hα)); eauto.
+             apply (UB_mon_grading _ _
+                      (x1 + (SeriesC (λ ρ : language.state prob_lang, language.state_step σ1 α ρ * x2 (e1, ρ))))) => //.
+             eapply ub_lift_dbind_adv; eauto; [by destruct x1|].
+             destruct Hx'' as [r Hr]; exists r.
+             intros a.
+             split; [by destruct (x2 _) | by apply Hr].
+           - iIntros (e s).
+             iApply step_fupd_fupdN_S.
+             iMod ("H" with "[//]") as "H"; iModIntro.
+             iDestruct "H" as "[%R' [%x1' [%x2' (%Hsum' & %Hlift' & Hwand')]]]".
+             rewrite -(dret_id_left' (fun _ : () => (exec (S n) _)) tt).
+             iApply (step_fupdN_mono _ _ _ ⌜(ub_lift _ _ (x1' + x2')) ⌝).
+             { iIntros "%H'"; iPureIntro. eapply UB_mon_grading; eauto. }
+             iApply (ub_lift_dbind').
+             * iPureIntro; apply cond_nonneg.
+             * iPureIntro; apply cond_nonneg.
+             * iPureIntro.
+               apply total_ub_lift_implies_ub_lift in Hlift'.
+               eapply Hlift'.
+             * iIntros (? Hcont).
+               replace tt with a; [| by destruct a].
+               iSpecialize ("Hwand'" with "[]"); [iPureIntro; eauto|].
+               rewrite (dret_id_left').
+               iApply step_fupd_fupdN_S.
+               iMod ("Hwand'" with "[//]"); iModIntro; iFrame.
+               iModIntro; eauto. }
+         iInduction (language.get_active σ1) as [| α] "IH"; [done|].
+         rewrite big_orL_cons.
+         iDestruct "H" as "[H | Ht]"; [done|].
+         by iApply "IH".
+     Qed. *)
+
+  Theorem wp_refRcoupl_step_fupdN (e : expr) (σ : state) (x : nonnegreal) n φ  :
+    state_interp σ ∗ etc_interp (x) ∗ WP e {{ v, ⌜φ v⌝ }} ⊢
+    |={⊤,∅}=> |={∅}▷=>^n ⌜ERT n (e, σ) <= x⌝.
+  Proof.
+    iInduction n as [|n] "IH" forall (e σ x); iIntros "((Hσh & Hσt) & Hx & Hwp)".
+    - simpl.
+      iApply fupd_mask_intro; [set_solver|]; iIntros.
+      iPureIntro. apply cond_nonneg.
+    - iSimpl.
+      destruct (to_val e) eqn:Heq.
+      + iApply fupd_mask_intro; [set_solver|]; iIntros "_".
         iApply step_fupdN_intro; [done|]. do 4 iModIntro.
         iPureIntro.
-        rewrite exec_unfold dret_id_left /=.
-        apply (UB_mon_grading _ _ 0); [apply cond_nonneg | ].
-        apply ub_lift_dret; auto.
-      + rewrite ub_wp_unfold /ub_wp_pre /= Heq.
+        apply cond_nonneg.
+      + rewrite ert_wp_unfold /ert_wp_pre /= Heq.
         iMod ("Hwp" with "[$]") as "Hlift".
         iModIntro.
         iPoseProof
-          (exec_ub_mono _ (λ '(e2, σ2) ε', |={∅}▷=>^(S n)
-             ⌜ub_lift (exec n (e2, σ2)) φ ε'⌝)%I
+          (ERM_mono _ (λ '(e2, σ2) x', |={∅}▷=>^(S n)
+             ⌜ERT n (e2, σ2) <= x'⌝)%I
             with "[%] [] Hlift") as "H".
         { apply Rle_refl. }
         { iIntros ([] ?) "H !> !>".
           iMod "H" as "(Hstate & Herr_auth & Hwp)".
           iMod ("IH" with "[$]") as "H".
           iModIntro. done. }
-        assert ((prim_step e σ) = (step (e, σ))) as h => //.
-        rewrite h. clear h.
-        rewrite -exec_Sn_not_final; [|eauto].
-        iAssert
-          (|={∅}▷=> |={∅}▷=>^n ⌜ub_lift (exec (S n) (e, σ)) φ ε⌝)%I
-          with "[H]" as "Haux"; last first.
-        {  iMod "Haux".
-           do 2 iModIntro.
-           iMod "Haux".
-           iModIntro.
-           iApply (step_fupdN_wand with "Haux").
-           iPureIntro; done.
-         }
-        by iApply (exec_ub_erasure with "H").
+        assert ((prim_step e σ) = (step (e, σ))) as -> => //.
+        rewrite -ERT_Sn => //.
+        by iApply (ERM_erasure with "H").
   Qed.
-*)
+
 
 End adequacy.
 
-(*
-Class ub_clutchGpreS Σ := UB_ClutchGpreS {
-  ub_clutchGpreS_iris  :: invGpreS Σ;
-  ub_clutchGpreS_heap  :: ghost_mapG Σ loc val;
-  ub_clutchGpreS_tapes :: ghost_mapG Σ loc tape;
-  ub_clutchGpreS_err   :: ecGpreS Σ;
+
+Class ert_clutchGpreS Σ := ERT_ClutchGpreS {
+  ert_clutchGpreS_iris  :: invGpreS Σ;
+  ert_clutchGpreS_heap  :: ghost_mapG Σ loc val;
+  ert_clutchGpreS_tapes :: ghost_mapG Σ loc tape;
+  ert_clutchGpreS_etc   :: etcGpreS Σ;
 }.
 
-Definition ub_clutchΣ : gFunctors :=
+Definition ert_clutchΣ : gFunctors :=
   #[invΣ; ghost_mapΣ loc val;
     ghost_mapΣ loc tape;
-    GFunctor (authR (realUR))].
-Global Instance subG_ub_clutchGPreS {Σ} : subG ub_clutchΣ Σ → ub_clutchGpreS Σ.
+    GFunctor (authR (nonnegrealUR))].
+Global Instance subG_ert_clutchGPreS {Σ} : subG ert_clutchΣ Σ → ert_clutchGpreS Σ.
 Proof. solve_inG. Qed.
 
-Theorem wp_union_bound Σ `{ub_clutchGpreS Σ} (e : expr) (σ : state) n (ε : nonnegreal) φ :
-  (∀ `{ub_clutchGS Σ}, ⊢ € ε -∗ WP e {{ v, ⌜φ v⌝ }}) →
-  ub_lift (exec n (e, σ)) φ ε.
+Theorem wp_ERT Σ `{ert_clutchGpreS Σ} (e : expr) (σ : state) n (x : nonnegreal) φ :
+  (∀ `{ert_clutchGS Σ}, ⊢ ⧖ x -∗ WP e {{ v, ⌜φ v⌝ }}) →
+  ERT n (e, σ) <= x.
 Proof.
   intros Hwp.
   eapply pure_soundness, (step_fupdN_soundness_no_lc _ n 0).
@@ -244,16 +293,16 @@ Proof.
   iMod (ghost_map_alloc σ.(heap)) as "[%γH [Hh _]]".
   iMod (ghost_map_alloc σ.(tapes)) as "[%γT [Ht _]]".
   (* Handle the trivial 1 <= ε case *)
-  destruct (Rlt_decision (nonneg ε) 1) as [Hcr|Hcr]; last first.
-  { iClear "Hh Ht".
-    iApply (fupd_mask_intro); [eauto|].
-    iIntros "_".
-    iApply step_fupdN_intro; [eauto|].
-    iApply laterN_intro; iPureIntro.
-    apply not_Rlt, Rge_le in Hcr.
-    rewrite /ub_lift; intros.
-    eapply Rle_trans; [eapply prob_le_1|done]. }
-  iMod (ec_alloc with "[//]") as (?) "[? ?]".
+  (* destruct (Rlt_decision (nonneg ε) 1) as [Hcr|Hcr]; last first.
+     { iClear "Hh Ht".
+       iApply (fupd_mask_intro); [eauto|].
+       iIntros "_".
+       iApply step_fupdN_intro; [eauto|].
+       iApply laterN_intro; iPureIntro.
+       apply not_Rlt, Rge_le in Hcr.
+       rewrite /ub_lift; intros.
+       eapply Rle_trans; [eapply prob_le_1|done]. } *)
+  iMod (etc_alloc) as (?) "[??]".
   set (HclutchGS := HeapG Σ _ _ _ γH γT _).
   iApply wp_refRcoupl_step_fupdN.
   iFrame.
@@ -261,6 +310,7 @@ Proof.
   done.
 Qed.
 
+(*
 Lemma ub_lift_closed_lim (e : expr) (σ : state) (ε : nonnegreal) φ :
   (forall n, ub_lift (exec n (e, σ)) φ ε ) ->
   ub_lift (lim_exec (e, σ)) φ ε .
