theories/ert_logic/ert_rules.v
@@ -4,9 +4,9 @@ From iris.proofmode Require Import proofmode.
 From clutch.prelude Require Import stdpp_ext.
 From clutch.prob_lang Require Import notation tactics metatheory.
 From clutch.prob_lang Require Export lang.
-From clutch.ub_logic Require Export lifting proofmode ectx_lifting primitive_laws seq_amplification.
+(* From clutch.ub_logic Require Export lifting proofmode ectx_lifting primitive_laws seq_amplification. *)
 
-Section metatheory.
+(* Section metatheory.
 
-  Local Open Scope R.
-End metatheory.
+     Local Open Scope R.
+   End metatheory. *)
